Security spec fixes.

verified/sec_prop.s.dfy
@@ -39,73 +39,90 @@ predicate pgInEnc(d: PageDb, n: PageNr, enc: PageNr)
 // 2. Public pages.
 // 3. (A subset of the) registers *only* when the malicious enclave is executing.
 
+// Our equivalent of an enclave number is a dispatcher page.
+
 // Low-equivalence relation that relates two PageDbs that appear equivalent to 
-// an attacker that controls an enclave in addrspace "atkr". 
+// an attacker that controls an enclave "atkr". 
 predicate enc_enc_conf_eqpdb(d1:PageDb, d2: PageDb, atkr:PageNr)
     requires validPageDb(d1) && validPageDb(d2)
     requires valDispPage(d1, atkr)
 {
     var atkr_asp := d1[atkr].addrspace;
+    // The disp page is the same in both states
     valDispPage(d2, atkr) &&
     d1[atkr].addrspace == d2[atkr].addrspace &&
-    valAddrPage(d1, atkr) && valAddrPage(d2, atkr) &&
-    (forall n : PageNr :: pgInAddrSpc(d1, n, atkr) <==>
-        pgInAddrSpc(d2, n, atkr)) &&
-    (forall n : PageNr | pgInAddrSpc(d1, n, atkr) ::
-        d2[n].PageDbEntryTyped? && d1[n].entry == d2[n].entry)
+    // The addrspace is an addrspace page in both states
+    valAddrPage(d1, atkr_asp) && valAddrPage(d2, atkr_asp) &&
+    // The set of pages that belong to the enclave is the same in both 
+    // states.
+    (forall n : PageNr :: pgInAddrSpc(d1, n, atkr_asp) <==>
+        pgInAddrSpc(d2, n, atkr_asp)) &&
+    // This together with two concrete states that refine d1, d2 ensure that 
+    // the contents of the pages that belong to the enclave are the same in 
+    // both states.
+    (forall n : PageNr | pgInAddrSpc(d1, n, atkr_asp) ::
+        d1[n].entry == d2[n].entry)
 }
 
 // Low-equivalence relation that relates two concrete states that appear 
-// equivalent to an attacker that controls an enclave in adddrspace "atkr". 
+// equivalent to an attacker that controls an enclave "atkr". 
 // A malicous attacker cannot observe anything when it is not executing (but it 
 // can always observe whether or not it is executing).
 //
 // The plan is to only check low-equivalence of states on entry/exit of 
-// the enclave so this only needs to hold then.
+// the enclave so this only needs to hold then. This equivalence relation need 
+// not hold for smc calls other than enter/resume.
 predicate enc_enc_conf_eq(s1:state, s2:state, d1:PageDb, d2:PageDb, 
     atkr:PageNr)
     requires SaneState(s1) && SaneState(s2)
     requires validPageDb(d1) && validPageDb(d2)
-     requires pageDbCorresponds(s1.m, d1) && pageDbCorresponds(s2.m, d2)
+    requires pageDbCorresponds(s1.m, d1) && pageDbCorresponds(s2.m, d2)
     requires valDispPage(d1, atkr)
     requires valAddrPage(d1, d1[atkr].addrspace)
     requires enc_enc_conf_eqpdb(d1, d2, atkr)
 {
     var atkr_asp := d1[atkr].addrspace;
     var l1p := d1[atkr_asp].entry.l1ptnr; // same in both d1, d2 because of eqdb
-    regs_usr_equiv(s1.regs, s2.regs) &&
-    configs_usr_equiv(s1.conf, s2.conf) &&
+    regs_usr_equiv(s1, s2) &&
+    configs_usr_equiv(s1, s2) &&
+    nonStoppedL1(d1, l1p) <==> nonStoppedL1(d2, l1p) &&
     nonStoppedL1(d1, l1p) ==>
         (PagesInTable(mkAbsPTable(d1, l1p)) == 
             PagesInTable(mkAbsPTable(d2, l1p)))
 
 }
 
-predicate regs_usr_equiv(r1:map<ARMReg,word>, r2:map<ARMReg,word>)
-    requires ValidRegState(r1) && ValidRegState(r2)
+predicate regs_usr_equiv(s1:state, s2:state)
+    requires SaneState(s1) && SaneState(s2)
 {
     reveal_ValidRegState();
-    r1[R0]  == r2[R0] &&
-    r1[R1]  == r2[R1] &&
-    r1[R2]  == r2[R2] &&
-    r1[R3]  == r2[R3] &&
-    r1[R4]  == r2[R4] &&
-    r1[R5]  == r2[R5] &&
-    r1[R6]  == r2[R6] &&
-    r1[R7]  == r2[R7] &&
-    r1[R8]  == r2[R8] &&
-    r1[R9]  == r2[R9] &&
-    r1[R10] == r2[R10] &&
-    r1[R11] == r2[R11] &&
-    r1[R12] == r2[R12] &&
-    r1[SP(User)] == r2[SP(User)] &&
-    r1[LR(User)] == r2[LR(User)]
+    reveal_ValidSRegState();
+    OperandContents(s1, OReg(R0))  == OperandContents(s2, OReg(R0)) &&
+    OperandContents(s1, OReg(R1))  == OperandContents(s2, OReg(R1)) &&
+    OperandContents(s1, OReg(R2))  == OperandContents(s2, OReg(R2)) &&
+    OperandContents(s1, OReg(R3))  == OperandContents(s2, OReg(R3)) &&
+    OperandContents(s1, OReg(R4))  == OperandContents(s2, OReg(R4)) &&
+    OperandContents(s1, OReg(R5))  == OperandContents(s2, OReg(R5)) &&
+    OperandContents(s1, OReg(R6))  == OperandContents(s2, OReg(R6)) &&
+    OperandContents(s1, OReg(R7))  == OperandContents(s2, OReg(R7)) &&
+    OperandContents(s1, OReg(R8))  == OperandContents(s2, OReg(R8)) &&
+    OperandContents(s1, OReg(R9))  == OperandContents(s2, OReg(R9)) &&
+    OperandContents(s1, OReg(R10)) == OperandContents(s2, OReg(R10)) &&
+    OperandContents(s1, OReg(R11)) == OperandContents(s2, OReg(R11)) &&
+    OperandContents(s1, OReg(R12)) == OperandContents(s2, OReg(R12)) &&
+    // This contains the PC on both entry and exit from the enclave.
+    OperandContents(s1, OLR) == OperandContents(s2, OLR)
 }
 
-predicate configs_usr_equiv(c1:config, c2:config)
+predicate configs_usr_equiv(s1:state, s2: state)
+    requires SaneState(s1) && SaneState(s2)
 {
-    // AFAIK nothing is visible in usermode
-    true
+    reveal_ValidRegState();
+    reveal_ValidSRegState();
+    // Using s.conf to determine whether or not the CPSR is equivalent would be 
+    // insufficient here because a user process can read the value of the 
+    // CPSR but the Config only models parts of the CPSR.
+    OperandContents(s1, OSReg(cpsr)) == OperandContents(s2, OSReg(cpsr))
 }
 
 // Like WritablePagesInTable but includes pages without the write bit set
