verified/sec_prop.i.dfy
@@ -9,13 +9,20 @@ lemma enter_enc_enc_conf_ni(s1: state, d1: PageDb, s1':state, d1': PageDb,
     requires SaneState(s1) && validPageDb(d1) && SaneState(s1') && validPageDb(d1')
     requires SaneState(s2) && validPageDb(d2) && SaneState(s2') && validPageDb(d2')
     requires pageDbCorresponds(s1.m, d1) && pageDbCorresponds(s1'.m, d1') 
-    requires pageDbCorresponds(s1.m, d2) && pageDbCorresponds(s2'.m, d2') 
+    requires pageDbCorresponds(s2.m, d2) && pageDbCorresponds(s2'.m, d2') 
     requires validPageNr(dispPage) && valDispPage(d1, dispPage) // Error case??
+    requires validPageNr(dispPage) && valDispPage(d1', dispPage)
+    // If smc_enter(s1, d1) => (s1', d1')
     requires smc_enter(s1, d1, s1', d1', dispPage, arg1, arg2, arg3)
+    // and smc_enter(s2, d2) => (s2', d2')
     requires smc_enter(s2, d2, s2', d2', dispPage, arg1, arg2, arg3)
+    // s.t. (s1, d1) =_{disp} (s2, d2)
     requires enc_enc_conf_eqpdb(d1, d2, dispPage)
     requires enc_enc_conf_eq(s1, s2, d1, d2, dispPage)
+    // then (s1', d1') =_{disp} (s2', d2')
     ensures  enc_enc_conf_eqpdb(d1', d2', dispPage)
     ensures  enc_enc_conf_eq(s1', s2', d1', d2', dispPage)
 {
+    // TODO proveme
+    assume false;
 }
